## 4.7 More Powerful LR Parsers

### 4.7.1

> Construct the

> a) canonical LR, and

> b) LALR

> sets of items for grammar $$~S~\rightarrow~S~S~+~|~S~S~*~|~a$$ of Exercise 4.2.1.

[LR(1)](https://cyberzhg.github.io/toolbox/lr1?grammar=UyAtPiBTIFMgKwogICB8IFMgUyAqCiAgIHwgYQ==)

[LALR](https://cyberzhg.github.io/toolbox/lalr?grammar=UyAtPiBTIFMgKwogICB8IFMgUyAqCiAgIHwgYQ==)

### 4.7.2

> Repeat Exercise 4.7.1 for each of the (augmented) grammars of Exercise 4.2.2 (a) - (g).

> a) $$S~\rightarrow~0~S~1~|~0~1$$.

[LR(1)](https://cyberzhg.github.io/toolbox/lr1?grammar=UyAtPiAwIFMgMSB8IDAgMQ==)

[LALR](https://cyberzhg.github.io/toolbox/lalr?grammar=UyAtPiAwIFMgMSB8IDAgMQ==)

> b) $$S~\rightarrow~+~S~S~|~*~S~S~|~a$$.

[LR(1)](https://cyberzhg.github.io/toolbox/lr1?grammar=UyAtPiArIFMgUyB8ICogUyBTIHwgYQ==)

[LALR](https://cyberzhg.github.io/toolbox/lalr?grammar=UyAtPiArIFMgUyB8ICogUyBTIHwgYQ==)

> c) $$S~\rightarrow~S~(~S~)~S~|~\epsilon$$.

[LR(1)](https://cyberzhg.github.io/toolbox/lr1?grammar=UyAtPiBTICggUyApIFMgfCDPtQ==)

[LALR](https://cyberzhg.github.io/toolbox/lalr?grammar=UyAtPiBTICggUyApIFMgfCDPtQ==)

> d) $$S~\rightarrow~S~+~S~|~S~S~|~(~S~)|~S~*~|~a$$.

[LR(1)](https://cyberzhg.github.io/toolbox/lr1?grammar=UyAtPiBTICsgUyB8IFMgUyB8ICggUyApIHwgUyAqIHwgYQ==)

[LALR](https://cyberzhg.github.io/toolbox/lalr?grammar=UyAtPiBTICsgUyB8IFMgUyB8ICggUyApIHwgUyAqIHwgYQ==)

> e) $$S~\rightarrow~(~L~)~|~a$$ and $$L~\rightarrow~L~,~S~|~S~$$.

[LR(1)](https://cyberzhg.github.io/toolbox/lr1?grammar=UyAtPiAoIEwgKSB8IGEKTCAtPiBMICwgUyB8IFM=)

[LALR](https://cyberzhg.github.io/toolbox/lalr?grammar=UyAtPiAoIEwgKSB8IGEKTCAtPiBMICwgUyB8IFM=)

> f) $$S~\rightarrow~a~S~b~S~|~b~S~a~S~|~\epsilon$$.

[LR(1)](https://cyberzhg.github.io/toolbox/lr1?grammar=UyAtPiBhIFMgYiBTIHwgYiBTIGEgUyB8IM+1)

[LALR](https://cyberzhg.github.io/toolbox/lalr?grammar=UyAtPiBhIFMgYiBTIHwgYiBTIGEgUyB8IM+1)

> g) The following grammar for boolean expressions:

> $$
\begin{array}{rll}
bexpr &\rightarrow& bexpr~\mathbf{or}~bterm~|~bterm \\
bterm &\rightarrow& bterm~\mathbf{and}~bfactor~|~bfactor \\
bfactor &\rightarrow& \mathbf{not}~bfactor~|~(~bexpr~)~|~\mathbf{true}~|~\mathbf{false} \\
\end{array}
$$

[LR(1)](https://cyberzhg.github.io/toolbox/lr1?grammar=YmV4cHIgLT4gYmV4cHIgb3IgYnRlcm0gfCBidGVybSAKYnRlcm0gLT4gYnRlcm0gYW5kIGJmYWN0b3IgfCBiZmFjdG9yIApiZmFjdG9yIC0+IG5vdCBiZmFjdG9yIHwgKCBiZXhwciApIHwgdHJ1ZSB8IGZhbHNl)

[LALR](https://cyberzhg.github.io/toolbox/lalr?grammar=YmV4cHIgLT4gYmV4cHIgb3IgYnRlcm0gfCBidGVybSAKYnRlcm0gLT4gYnRlcm0gYW5kIGJmYWN0b3IgfCBiZmFjdG9yIApiZmFjdG9yIC0+IG5vdCBiZmFjdG9yIHwgKCBiZXhwciApIHwgdHJ1ZSB8IGZhbHNl)

### 4.7.3

### 4.7.4

> Show that the following grammar

> $$
\begin{array}{rll}
S&\rightarrow&A~a~|~b~A~c~|~d~c~|~b~d~a~\\
A&\rightarrow&d~\\
\end{array}
$$

> is LALR(1) but not SLR(1).

[LALR](https://cyberzhg.github.io/toolbox/lalr?grammar=UyAtPiBBIGEgfCBiIEEgYyB8IGQgYyB8IGIgZCBhCkEgLT4gZA==)

[SLR(1)](https://cyberzhg.github.io/toolbox/lr0?grammar=UyAtPiBBIGEgfCBiIEEgYyB8IGQgYyB8IGIgZCBhCkEgLT4gZA==)

### 4.7.5

> Show that the following grammar

> $$
\begin{array}{rll}
S&\rightarrow&A~a~|~b~A~c~|~B~c~|~b~B~a~\\
A&\rightarrow&d~\\
B&\rightarrow&d
\end{array}
$$

> is LR(1) but not LALR(1).

[LR(1)](https://cyberzhg.github.io/toolbox/lr1?grammar=UyAtPiBBIGEgfCBiIEEgYyB8IEIgYyB8IGIgQiBhCkEgLT4gZApCIC0+IGQ=)

[LALR(1)](https://cyberzhg.github.io/toolbox/lalr?grammar=UyAtPiBBIGEgfCBiIEEgYyB8IEIgYyB8IGIgQiBhCkEgLT4gZApCIC0+IGQ=)
